@prefix : <http://fairmat-nfdi.eu/taxonomy/> .
@prefix owl: <http://www.w3.org/2002/07/owl#> .
@prefix rdf: <http://www.w3.org/1999/02/22-rdf-syntax-ns#> .
@prefix xml: <http://www.w3.org/XML/1998/namespace> .
@prefix xsd: <http://www.w3.org/2001/XMLSchema#> .
@prefix rdfs: <http://www.w3.org/2000/01/rdf-schema#> .
@base <http://fairmat-nfdi.eu/taxonomy/> .

<http://fairmat-nfdi.eu/taxonomy> rdf:type owl:Ontology .

#################################################################
#    Object Properties
#################################################################

###  http://fairmat-nfdi.eu/taxonomy/hasMaterialProperty
:hasMaterialProperty rdf:type owl:ObjectProperty ;
                     rdfs:subPropertyOf owl:topObjectProperty ;
                     rdfs:domain :Material ;
                     rdfs:range :MaterialProperty ;
                     rdfs:label "hasMaterialProperty"@en .


#################################################################
#    Classes
#################################################################

###  http://fairmat-nfdi.eu/taxonomy/AbsorptionCoefficient
:AbsorptionCoefficient rdf:type owl:Class ;
                       rdfs:subClassOf :OpticalProperty ;
                       rdfs:comment "a value representing how far into a material light of a particular wavelength can penetrate before it is absorbed"@en .


###  http://fairmat-nfdi.eu/taxonomy/Activity
:Activity rdf:type owl:Class ;
          rdfs:subClassOf :ThermophysicalProperty ;
          rdfs:comment "a measure of the effective concentration of a species under non-ideal (e.g., concentrated) conditions"@en .


###  http://fairmat-nfdi.eu/taxonomy/AnodicPartialCurrent
:AnodicPartialCurrent rdf:type owl:Class ;
                      rdfs:subClassOf :CorrosionProperty ;
                      rdfs:comment "sum of all the currents corresponding to anodic reactions on the electrode"@en .


###  http://fairmat-nfdi.eu/taxonomy/Area
:Area rdf:type owl:Class ;
      rdfs:subClassOf :StructuralProperty ;
      rdfs:comment "area of the specimen surface"@en .


###  http://fairmat-nfdi.eu/taxonomy/AxialForce
:AxialForce rdf:type owl:Class ;
            rdfs:subClassOf :VariableViscosity .


###  http://fairmat-nfdi.eu/taxonomy/BandGap
:BandGap rdf:type owl:Class ;
         rdfs:subClassOf :ElectricalProperty ;
         rdfs:comment "an energy range in a solid where no electronic states can exist (between valence band and conduction band)"@en .


###  http://fairmat-nfdi.eu/taxonomy/BetSurfaceArea
:BetSurfaceArea rdf:type owl:Class ;
                rdfs:subClassOf :StructuralProperty ;
                rdfs:comment "Brunauer-Emmett-Teller (BET) surface area of material_n"@en .


###  http://fairmat-nfdi.eu/taxonomy/BowingParameter
:BowingParameter rdf:type owl:Class ;
                 rdfs:subClassOf :ElectricalProperty ;
                 rdfs:comment "A parameter that decribes nonlinear variation of band gap between two materials with different lattice constants"@en .


###  http://fairmat-nfdi.eu/taxonomy/BulkModulus
:BulkModulus rdf:type owl:Class ;
             rdfs:subClassOf :MechanicalProperty ;
             rdfs:comment "measure of how resistant to compression that substance is"@en .


###  http://fairmat-nfdi.eu/taxonomy/BurgersVector
:BurgersVector rdf:type owl:Class ;
               rdfs:subClassOf :OneDDefect ;
               rdfs:comment "magnitude and direction of the lattice distortion resulting from a dislocation"@en .


###  http://fairmat-nfdi.eu/taxonomy/CarrierConcentration
:CarrierConcentration rdf:type owl:Class ;
                      rdfs:subClassOf :ElectricalProperty ;
                      rdfs:comment "number of charge carriers per volume"@en .


###  http://fairmat-nfdi.eu/taxonomy/CarrierDiffusionLength
:CarrierDiffusionLength rdf:type owl:Class ;
                        rdfs:subClassOf :ElectricalProperty ;
                        rdfs:comment "an average distance that the excess carriers can cover before they recombine"@en .


###  http://fairmat-nfdi.eu/taxonomy/CarrierLifetime
:CarrierLifetime rdf:type owl:Class ;
                 rdfs:subClassOf :ElectricalProperty ;
                 rdfs:comment "an average time it takes for a minority carrier to recombine"@en .


###  http://fairmat-nfdi.eu/taxonomy/CathodicPartialCurrent
:CathodicPartialCurrent rdf:type owl:Class ;
                        rdfs:subClassOf :CorrosionProperty ;
                        rdfs:comment "sum of all the currents corresponding to cathodic electochemical reactions on the electrode"@en .


###  http://fairmat-nfdi.eu/taxonomy/CharpyImpactEnergy
:CharpyImpactEnergy rdf:type owl:Class ;
                    rdfs:subClassOf :MechanicalProperty ;
                    rdfs:comment "work done to fracture a test specimen measured by Charpy impact test"@en .


###  http://fairmat-nfdi.eu/taxonomy/ChemicalPotential
:ChemicalPotential rdf:type owl:Class ;
                   rdfs:subClassOf :ThermophysicalProperty ;
                   rdfs:comment "rate of increase in the Gibbs free energy of the system with respect to the increase in the number of moles of species"@en .


###  http://fairmat-nfdi.eu/taxonomy/CoerciveElectricField
:CoerciveElectricField rdf:type owl:Class ;
                       rdfs:subClassOf :FerroelectricProperty ;
                       rdfs:comment "the strength of the electric field at which the macroscopic polarization of the ferroelectric capacitor disappears, presented by values assigned to symbols E_{c}"@en .


###  http://fairmat-nfdi.eu/taxonomy/CoersiveField
:CoersiveField rdf:type owl:Class ;
               rdfs:subClassOf :MagneticProperty ;
               rdfs:comment "The magnitude of the magnetic field in the opposite direction required to make the residual magnetism that remains even after applying a magnetic field to a ferromagnetic material to make it magentic until it becomes saturated and the reducing the magnetic field to zero again."@en .


###  http://fairmat-nfdi.eu/taxonomy/Color
:Color rdf:type owl:Class ;
       rdfs:subClassOf :OpticalProperty ;
       rdfs:comment "color of a material"@en .


###  http://fairmat-nfdi.eu/taxonomy/Composition
:Composition rdf:type owl:Class ;
             rdfs:subClassOf :StructuralProperty ;
             rdfs:comment "elemental constituent of phase_n"@en .


###  http://fairmat-nfdi.eu/taxonomy/Compressibility
:Compressibility rdf:type owl:Class ;
                 rdfs:subClassOf :MechanicalProperty ;
                 rdfs:comment "reciprocal of bulk modulus"@en .


###  http://fairmat-nfdi.eu/taxonomy/CompressiveProperty
:CompressiveProperty rdf:type owl:Class ;
                     rdfs:subClassOf :MechanicalProperty ;
                     rdfs:comment "properties indicate how the material will react to forces being applied in compression"@en .


###  http://fairmat-nfdi.eu/taxonomy/CorrosionCurrent
:CorrosionCurrent rdf:type owl:Class ;
                  rdfs:subClassOf :CorrosionProperty ;
                  rdfs:comment "anodic partial current due to metal oxidation"@en .


###  http://fairmat-nfdi.eu/taxonomy/CorrosionPotential
:CorrosionPotential rdf:type owl:Class ;
                    rdfs:subClassOf :CorrosionProperty ;
                    rdfs:comment "electrode potential of a metal in a given corrosion system"@en .


###  http://fairmat-nfdi.eu/taxonomy/CorrosionProperty
:CorrosionProperty rdf:type owl:Class ;
                   rdfs:subClassOf :MaterialProperty ;
                   rdfs:comment "properties related to deterioration of a material as it reacts with its envirionment via electrochemical and chemical reactions"@en .


###  http://fairmat-nfdi.eu/taxonomy/CorrosionRate
:CorrosionRate rdf:type owl:Class ;
               rdfs:subClassOf :CorrosionProperty ;
               rdfs:comment "amount of corrosion loss per year in thckness"@en .


###  http://fairmat-nfdi.eu/taxonomy/Crack_tip_opening_displacement
:Crack_tip_opening_displacement rdf:type owl:Class ;
                                rdfs:subClassOf :MechanicalProperty ;
                                rdfs:comment "\"crack displacement resulting from the total deformation at variously defined locations near the original crack tip\"" .


###  http://fairmat-nfdi.eu/taxonomy/CreepProperty
:CreepProperty rdf:type owl:Class ;
               rdfs:subClassOf :MechanicalProperty ;
               rdfs:comment "materials response upon long-term exposure to high levels of stress that are still below the yield strength of the materials"@en .


###  http://fairmat-nfdi.eu/taxonomy/CreepRuptureStrain
:CreepRuptureStrain rdf:type owl:Class ;
                    rdfs:subClassOf :MechanicalProperty ;
                    rdfs:comment "total strain after creep rupture test"@en .


###  http://fairmat-nfdi.eu/taxonomy/CreepRuptureStrength
:CreepRuptureStrength rdf:type owl:Class ;
                      rdfs:subClassOf :MechanicalProperty ;
                      rdfs:comment "stress causing fracture in a creep test at a given time, in a specified constant environment"@en .


###  http://fairmat-nfdi.eu/taxonomy/CriticalResolvedShearStress
:CriticalResolvedShearStress rdf:type owl:Class ;
                             rdfs:subClassOf :MechanicalProperty ;
                             rdfs:comment "component of shear stress necessary to initiate slip in a grain"@en .


###  http://fairmat-nfdi.eu/taxonomy/CryoscopicConstant
:CryoscopicConstant rdf:type owl:Class ;
                    rdfs:subClassOf :ThermophysicalProperty ;
                    rdfs:comment "elevation in boiling point produced when 1 mole of solute is dissolved in 1 kg of solvent"@en .


###  http://fairmat-nfdi.eu/taxonomy/CurieTemperature
:CurieTemperature rdf:type owl:Class ;
                  rdfs:subClassOf :MagneticProperty ;
                  rdfs:comment "temperature above which certain materials lose their permanent magnetic properties"@en .


###  http://fairmat-nfdi.eu/taxonomy/DBTransTemp
:DBTransTemp rdf:type owl:Class ;
             rdfs:subClassOf :MechanicalProperty ;
             rdfs:comment "temperature at which there is a pronounced decrease in a material’s ability to absorb force without fracturing"@en .


###  http://fairmat-nfdi.eu/taxonomy/DebyeTemperature
:DebyeTemperature rdf:type owl:Class ;
                  rdfs:subClassOf :ThermophysicalProperty ;
                  rdfs:comment "temperature of a crystal's highest normal mode of a vibration"@en .


###  http://fairmat-nfdi.eu/taxonomy/Defect
:Defect rdf:type owl:Class ;
        rdfs:subClassOf :StructuralProperty ;
        rdfs:comment "defect of materials ranging from 0D point defects to 2D interface"@en .


###  http://fairmat-nfdi.eu/taxonomy/Density
:Density rdf:type owl:Class ;
         rdfs:subClassOf :StructuralProperty ;
         rdfs:comment "mass per unit volum of a substance"@en .


###  http://fairmat-nfdi.eu/taxonomy/ZeroDDefectDensity
:ZeroDDefectDensity rdf:type owl:Class ;
                    rdfs:subClassOf :ZeroDDefect ;
                    rdfs:comment "ratio of defected lattice sites to those containig atoms"@en .


###  http://fairmat-nfdi.eu/taxonomy/OneDDefectDensity
:OneDDefectDensity rdf:type owl:Class ;
                   rdfs:subClassOf :OneDDefect ;
                   rdfs:comment "measure of the number of dislocations in a unit volume of a crystalline material"@en .


###  http://fairmat-nfdi.eu/taxonomy/DensityOfStates
:DensityOfStates rdf:type owl:Class ;
                 rdfs:subClassOf :ElectricalProperty ;
                 rdfs:comment "proportion of states that are to be occupied bsy the system at each energy, submitted in the form of file or array numeric data"@en .


###  http://fairmat-nfdi.eu/taxonomy/Diameter
:Diameter rdf:type owl:Class ;
          rdfs:subClassOf :Particle ;
          rdfs:comment "average diameter of spherical or rod shaped particles"@en .


###  http://fairmat-nfdi.eu/taxonomy/DielectricConstant
:DielectricConstant rdf:type owl:Class ;
                    rdfs:subClassOf :ElectricalProperty ;
                    rdfs:comment "relative premittivity compared to the vacuum in induced polarization stored in a material under electric field."@en .


###  http://fairmat-nfdi.eu/taxonomy/DielectricStrength
:DielectricStrength rdf:type owl:Class ;
                    rdfs:subClassOf :ElectricalProperty ;
                    rdfs:comment "the maximum electric field that the material can withstand under ideal conditions without undergoing electrical breakdown and becoming electrically conductive"@en .


###  http://fairmat-nfdi.eu/taxonomy/Diffusivity
:Diffusivity rdf:type owl:Class ;
             rdfs:subClassOf :ThermophysicalProperty ;
             rdfs:comment "the ratio of flux density to the negative of the concentration gradient in direction of diffusion"@en .


###  http://fairmat-nfdi.eu/taxonomy/Ecsa
:Ecsa rdf:type owl:Class ;
      rdfs:subClassOf :StructuralProperty ;
      rdfs:comment "electrochemically active surface area (ECSA) of material_n"@en .


###  http://fairmat-nfdi.eu/taxonomy/EffectiveVolume
:EffectiveVolume rdf:type owl:Class ;
                 rdfs:subClassOf :StructuralProperty ;
                 rdfs:comment "effective volume of the specimen"@en .


###  http://fairmat-nfdi.eu/taxonomy/ElasticProperty
:ElasticProperty rdf:type owl:Class ;
                 rdfs:subClassOf :MechanicalProperty ;
                 rdfs:comment "mechanical property of a material to withstand the compression or the elongation with respect to its length"@en .


###  http://fairmat-nfdi.eu/taxonomy/ElectricCharge
:ElectricCharge rdf:type owl:Class ;
                rdfs:subClassOf :ZeroDDefect ;
                rdfs:comment "charge state of point defecs in the unit of electron"@en .


###  http://fairmat-nfdi.eu/taxonomy/ElectricCurieTemperature
:ElectricCurieTemperature rdf:type owl:Class ;
                          rdfs:subClassOf :ElectricalProperty ;
                          rdfs:comment "temperature above which certain materials lose their permanent polarization properties"@en .


###  http://fairmat-nfdi.eu/taxonomy/ElectricSusceptibility
:ElectricSusceptibility rdf:type owl:Class ;
                        rdfs:subClassOf :ElectricalProperty ;
                        rdfs:comment "a dimensionless proportionality constant that indicates the degree of polarization of a material"@en .


###  http://fairmat-nfdi.eu/taxonomy/ElectricalConductivity
:ElectricalConductivity rdf:type owl:Class ;
                        rdfs:subClassOf :ElectricalProperty ;
                        rdfs:comment "quantity how strongly it conducts electric current"@en .


###  http://fairmat-nfdi.eu/taxonomy/ElectricalProperty
:ElectricalProperty rdf:type owl:Class ;
                    rdfs:subClassOf :MaterialProperty ;
                    rdfs:comment "physical properties that a material exhibits upon the application of electric forces"@en .


###  http://fairmat-nfdi.eu/taxonomy/ElectrochemPhaseStability
:ElectrochemPhaseStability rdf:type owl:Class ;
                           rdfs:subClassOf :ElectrochemicalProperty ;
                           rdfs:comment "the oxidation and reduction potential of solid or liquid materials (eg. the  solvent, the conductive salt or solid electrolytes)"@en .


###  http://fairmat-nfdi.eu/taxonomy/ElectrochemicalProperty
:ElectrochemicalProperty rdf:type owl:Class ;
                         rdfs:subClassOf :MaterialProperty ;
                         rdfs:comment "property either caused or accompanied by the passage of an electric current"@en .


###  http://fairmat-nfdi.eu/taxonomy/ElectromechanicalCouplingFactor
:ElectromechanicalCouplingFactor rdf:type owl:Class ;
                                 rdfs:subClassOf :PiezoelectricProperty ;
                                 rdfs:comment "conversion efficiency between electrical and mechanical energy,k^2"@en .


###  http://fairmat-nfdi.eu/taxonomy/ElectronEffectiveMass
:ElectronEffectiveMass rdf:type owl:Class ;
                       rdfs:subClassOf :ElectricalProperty ;
                       rdfs:comment "a mass that a particle seems to have when responding to forces or interacting with other identical particles in a thermal distribution"@en .


###  http://fairmat-nfdi.eu/taxonomy/ElectronMobility
:ElectronMobility rdf:type owl:Class ;
                  rdfs:subClassOf :ElectricalProperty ;
                  rdfs:comment "a value that represents how quickly a single electron can move through a metal or semiconductor, when pulled by an electric field"@en .


###  http://fairmat-nfdi.eu/taxonomy/EnthalpyOfFormation
:EnthalpyOfFormation rdf:type owl:Class ;
                     rdfs:subClassOf :ThermophysicalProperty ;
                     rdfs:comment "a measure of the energy released or consumed when one mole of a substance is created from its pure elements"@en .


###  http://fairmat-nfdi.eu/taxonomy/ExcitonBindingEnergy
:ExcitonBindingEnergy rdf:type owl:Class ;
                      rdfs:subClassOf :ElectricalProperty ;
                      rdfs:comment "a binding energy of an exciton (an electrically neutral quasiparticle that exists in insulators or semiconductors)"@en .


###  http://fairmat-nfdi.eu/taxonomy/Facet
:Facet rdf:type owl:Class ;
       rdfs:subClassOf :Particle ;
       rdfs:comment "facet orientation of the particle"@en .


###  http://fairmat-nfdi.eu/taxonomy/FatigueCrackGrowthRate
:FatigueCrackGrowthRate rdf:type owl:Class ;
                        rdfs:subClassOf :MechanicalProperty ;
                        rdfs:comment "rate of crack extension under fatigue loading, expressed in terms of crack extension per cycle, da/dN"@en .


###  http://fairmat-nfdi.eu/taxonomy/FatigueCrackGrowthThreshold
:FatigueCrackGrowthThreshold rdf:type owl:Class ;
                             rdfs:subClassOf :MechanicalProperty ;
                             rdfs:comment "asymptotic value of stress intensity factor range at which crack growth rate approaches zero"@en .


###  http://fairmat-nfdi.eu/taxonomy/FatigueLife
:FatigueLife rdf:type owl:Class ;
             rdfs:subClassOf :MechanicalProperty ;
             rdfs:comment "number of stress (strain) cyclcles required to cause failure"@en .


###  http://fairmat-nfdi.eu/taxonomy/FatigueLimit
:FatigueLimit rdf:type owl:Class ;
              rdfs:subClassOf :MechanicalProperty ;
              rdfs:comment "the highest stress that materials can withstand for an infinite number of cycles without breaking"@en .


###  http://fairmat-nfdi.eu/taxonomy/FatigueProperty
:FatigueProperty rdf:type owl:Class ;
                 rdfs:subClassOf :MechanicalProperty ;
                 rdfs:comment "materials response when subjected to cyclic load and/or strain"@en .


###  http://fairmat-nfdi.eu/taxonomy/FatiguePropertyType
:FatiguePropertyType rdf:type owl:Class ;
                     rdfs:subClassOf :MechanicalProperty ;
                     rdfs:comment "type of fatigue properties depending on number of cycles, applied stress and/or strain level and environment"@en .


###  http://fairmat-nfdi.eu/taxonomy/FermiLevel
:FermiLevel rdf:type owl:Class ;
            rdfs:subClassOf :ElectricalProperty ;
            rdfs:comment "the thermodynamic work required to add one electron to the body"@en .


###  http://fairmat-nfdi.eu/taxonomy/FerroelectricProperty
:FerroelectricProperty rdf:type owl:Class ;
                       rdfs:subClassOf :MaterialProperty ;
                       rdfs:comment "property of certain materials to have a spontaneous polarization which can be reversed by the application of an external electric field"@en .


###  http://fairmat-nfdi.eu/taxonomy/FormationEnergy
:FormationEnergy rdf:type owl:Class ;
                 rdfs:subClassOf :ZeroDDefect ;
                 rdfs:comment "defect formation energy, i.e. lattice cohesive energy in the case of vacancy"@en .


###  http://fairmat-nfdi.eu/taxonomy/Fraction
:Fraction rdf:type owl:Class ;
          rdfs:subClassOf :StructuralProperty ;
          rdfs:comment "relative amounts of phase_n in the microstructure"@en .


###  http://fairmat-nfdi.eu/taxonomy/FractureToughness
:FractureToughness rdf:type owl:Class ;
                   rdfs:subClassOf :MechanicalProperty ;
                   rdfs:comment "generic term for measures of resistance to extension of a crack"@en .


###  http://fairmat-nfdi.eu/taxonomy/FreeCorrosionCurrent
:FreeCorrosionCurrent rdf:type owl:Class ;
                      rdfs:subClassOf :CorrosionProperty ;
                      rdfs:comment "corrosion current at the free corrosion potential"@en .


###  http://fairmat-nfdi.eu/taxonomy/FreeCorrosionPotential
:FreeCorrosionPotential rdf:type owl:Class ;
                        rdfs:subClassOf :CorrosionProperty ;
                        rdfs:comment "corrosion potential in the absence of net (external) electrical current flowing to or from the metal surface"@en .


###  http://fairmat-nfdi.eu/taxonomy/Fugacity
:Fugacity rdf:type owl:Class ;
          rdfs:subClassOf :ThermophysicalProperty ;
          rdfs:comment "a measure of the effective pressure of a species in a real gas"@en .


###  http://fairmat-nfdi.eu/taxonomy/GibbsFreeEnergy
:GibbsFreeEnergy rdf:type owl:Class ;
                 rdfs:subClassOf :ThermophysicalProperty ;
                 rdfs:comment "a measure of the potential for reversible or maximum work that may be done by a system at constant temperature and pressure"@en .


###  http://fairmat-nfdi.eu/taxonomy/Grain
:Grain rdf:type owl:Class ;
       rdfs:subClassOf :StructuralProperty ;
       rdfs:comment "inner structure of material made of individual crystalline areas"@en .


###  http://fairmat-nfdi.eu/taxonomy/GrainAspectRatio
:GrainAspectRatio rdf:type owl:Class ;
                  rdfs:subClassOf :StructuralProperty ;
                  rdfs:comment "length ratio between longest distance and shortest distance of grain"@en .


###  http://fairmat-nfdi.eu/taxonomy/GrainSize
:GrainSize rdf:type owl:Class ;
           rdfs:subClassOf :StructuralProperty ;
           rdfs:comment "estimate of the average grain diameter"@en .


###  http://fairmat-nfdi.eu/taxonomy/HallCoefficient
:HallCoefficient rdf:type owl:Class ;
                 rdfs:subClassOf :ElectricalProperty ;
                 rdfs:comment "the ratio of the induced electric field to the product of the current density and the applied magnetic field"@en .


###  http://fairmat-nfdi.eu/taxonomy/HallVoltage
:HallVoltage rdf:type owl:Class ;
             rdfs:subClassOf :ElectricalProperty ;
             rdfs:comment "Voltage difference across an electrical conductor that is transverse to an electric current in the conductor and to an applied magnetic field perpendicular to the current"@en .


###  http://fairmat-nfdi.eu/taxonomy/Hardness
:Hardness rdf:type owl:Class ;
          rdfs:subClassOf :MechanicalProperty ;
          rdfs:comment "measure of the resistance to localized plastic deformation induced by either mechanical indentation or abrasion"@en .


###  http://fairmat-nfdi.eu/taxonomy/HeatCapacity
:HeatCapacity rdf:type owl:Class ;
              rdfs:subClassOf :ThermophysicalProperty ;
              rdfs:comment "quantity of heat necessary to change the temperature of an entity, substance or system by one Kelvin of temperature"@en .


###  http://fairmat-nfdi.eu/taxonomy/HeatOfFusion
:HeatOfFusion rdf:type owl:Class ;
              rdfs:subClassOf :ThermophysicalProperty ;
              rdfs:comment "heat absorbed by a unit mass of a solid at its melting point"@en .


###  http://fairmat-nfdi.eu/taxonomy/Height
:Height rdf:type owl:Class ;
        rdfs:subClassOf :Particle ;
        rdfs:comment "average height of particles"@en .


###  http://fairmat-nfdi.eu/taxonomy/HoleEffectiveMass
:HoleEffectiveMass rdf:type owl:Class ;
                   rdfs:subClassOf :ElectricalProperty ;
                   rdfs:comment "a mass that a particle seems to have when responding to forces or interacting with other identical particles in a thermal distribution"@en .


###  http://fairmat-nfdi.eu/taxonomy/HoleMobility
:HoleMobility rdf:type owl:Class ;
              rdfs:subClassOf :ElectricalProperty ;
              rdfs:comment "a value that represents how quickly a single hole can move through a metal or semiconductor, when pulled by an electric field"@en .


###  http://fairmat-nfdi.eu/taxonomy/ImpactToughness
:ImpactToughness rdf:type owl:Class ;
                 rdfs:subClassOf :MechanicalProperty ;
                 rdfs:comment "toughness of a material using the value of impact energy absorbed by the maerial during fracturing under impact"@en .


###  http://fairmat-nfdi.eu/taxonomy/Impurity
:Impurity rdf:type owl:Class ;
          rdfs:subClassOf :StructuralProperty ;
          rdfs:comment "impurities in the materials"@en .


###  http://fairmat-nfdi.eu/taxonomy/InitialVolume
:InitialVolume rdf:type owl:Class ;
               rdfs:subClassOf :StructuralProperty ;
               rdfs:comment "initial volume of the specimen"@en .


###  http://fairmat-nfdi.eu/taxonomy/InstantaneousStrain
:InstantaneousStrain rdf:type owl:Class ;
                     rdfs:subClassOf :MechanicalProperty ;
                     rdfs:comment "immediate deformation of materials upon initial application of a stress"@en .


###  http://fairmat-nfdi.eu/taxonomy/InterfacialEnergy
:InterfacialEnergy rdf:type owl:Class ;
                   rdfs:subClassOf :TwoDDefect ;
                   rdfs:comment "energy required to form a unit area of new interface"@en .


###  http://fairmat-nfdi.eu/taxonomy/IonicConductivity
:IonicConductivity rdf:type owl:Class ;
                   rdfs:subClassOf :ElectricalProperty ;
                   rdfs:comment "quantity how strongly it conducts ionic charge"@en .


###  http://fairmat-nfdi.eu/taxonomy/IonicMobility
:IonicMobility rdf:type owl:Class ;
               rdfs:subClassOf :ElectricalProperty ;
               rdfs:comment "The proportionality factor between an ion's drift velocity in an electric field in a specified medium"@en .


###  http://fairmat-nfdi.eu/taxonomy/JIC
:JIC rdf:type owl:Class ;
     rdfs:subClassOf :MechanicalProperty ;
     rdfs:comment "crack-extension resistance under conditions of crack-tip plane strain in mode I and substantial plastic deformation"@en .


###  http://fairmat-nfdi.eu/taxonomy/KIC
:KIC rdf:type owl:Class ;
     rdfs:subClassOf :MechanicalProperty ;
     rdfs:comment "crack-extension resistance under conditions of crack-tip plane strain in mode I and predominantly linear-elastic conditions"@en .


###  http://fairmat-nfdi.eu/taxonomy/LangmuirSurfaceArea
:LangmuirSurfaceArea rdf:type owl:Class ;
                     rdfs:subClassOf :StructuralProperty ;
                     rdfs:comment "Langmuir surface area of material_n"@en .


###  http://fairmat-nfdi.eu/taxonomy/LayerThickness
:LayerThickness rdf:type owl:Class ;
                rdfs:subClassOf :StructuralProperty ;
                rdfs:comment "layer thickness of the top contact layer material(n)"@en .


###  http://fairmat-nfdi.eu/taxonomy/Length
:Length rdf:type owl:Class ;
        rdfs:subClassOf :Particle ;
        rdfs:comment "length of the encapsulation layer"@en .


###  http://fairmat-nfdi.eu/taxonomy/LossModulus
:LossModulus rdf:type owl:Class ;
             rdfs:subClassOf :VariableViscosity .


###  http://fairmat-nfdi.eu/taxonomy/LowerShelfEnergy
:LowerShelfEnergy rdf:type owl:Class ;
                  rdfs:subClassOf :MechanicalProperty ;
                  rdfs:comment "low fracture energy associated with brittle behavior"@en .


###  http://fairmat-nfdi.eu/taxonomy/MagneticAnisotropyConstant
:MagneticAnisotropyConstant rdf:type owl:Class ;
                            rdfs:subClassOf :MagneticProperty ;
                            rdfs:comment "A measure of the energy density difference in magnetization depending on the direction when a magnetic material is magnetized by applying a magnetic field having an arbitrary direciton"@en .


###  http://fairmat-nfdi.eu/taxonomy/MagneticAnisotropyField
:MagneticAnisotropyField rdf:type owl:Class ;
                         rdfs:subClassOf :MagneticProperty ;
                         rdfs:comment "Magnetic field required for complete magnetization in the direction in which the largest magnetic field is required for magnetization in a magnetic material having magentic anisotropy"@en .


###  http://fairmat-nfdi.eu/taxonomy/MagneticHysteresis
:MagneticHysteresis rdf:type owl:Class ;
                    rdfs:subClassOf :MagneticProperty ;
                    rdfs:comment "When an external magnetic field is applied to a ferromagnetic material to continuously change its strength and direction, a graph representing the relationship between magnetic field and magnetization draws a closed magnetization curve"@en .


###  http://fairmat-nfdi.eu/taxonomy/MagneticProperty
:MagneticProperty rdf:type owl:Class ;
                  rdfs:subClassOf :MaterialProperty ;
                  rdfs:comment "physical properties that a material exhibits upon the application of magnetic forces"@en .


###  http://fairmat-nfdi.eu/taxonomy/Material
:Material rdf:type owl:Class ;
          rdfs:comment "description of material to be milled"@en .


###  http://fairmat-nfdi.eu/taxonomy/MaterialProperty
:MaterialProperty rdf:type owl:Class .


###  http://fairmat-nfdi.eu/taxonomy/MaxCompressiveStrength
:MaxCompressiveStrength rdf:type owl:Class ;
                        rdfs:subClassOf :MechanicalProperty ;
                        rdfs:comment "maximum compressive strength of material during compressive test"@en .


###  http://fairmat-nfdi.eu/taxonomy/MaximumEnergyProduct
:MaximumEnergyProduct rdf:type owl:Class ;
                      rdfs:subClassOf :MagneticProperty ;
                      rdfs:comment "The maximum energy product is defined based on the magnetic hysteresis saturation loop (B-H curve), in the demagnetizing portion where the B and H fields are in opposition. It is defined as the maximal value of the product of B and H along this curve"@en .


###  http://fairmat-nfdi.eu/taxonomy/MechanicalProperty
:MechanicalProperty rdf:type owl:Class ;
                    rdfs:subClassOf :MaterialProperty ;
                    rdfs:comment "physical properties that a material exhibits upon the application of forces"@en .


###  http://fairmat-nfdi.eu/taxonomy/MechanicalQualityFactor
:MechanicalQualityFactor rdf:type owl:Class ;
                         rdfs:subClassOf :PiezoelectricProperty ;
                         rdfs:comment "Variables that indicate how little loss is in piezoelectric deformation (It is the inverse of the mechanical loss tan ϕ)"@en .


###  http://fairmat-nfdi.eu/taxonomy/MeltingRange
:MeltingRange rdf:type owl:Class ;
              rdfs:subClassOf :ThermophysicalProperty ;
              rdfs:comment "temperature defference between liquidus and solidus at a given composition"@en .


###  http://fairmat-nfdi.eu/taxonomy/MeltingTemperature
:MeltingTemperature rdf:type owl:Class ;
                    rdfs:subClassOf :ThermophysicalProperty ;
                    rdfs:comment "temperature at the materials melt"@en .


###  http://fairmat-nfdi.eu/taxonomy/MinimumCreepRate
:MinimumCreepRate rdf:type owl:Class ;
                  rdfs:subClassOf :MechanicalProperty ;
                  rdfs:comment "slope of the portion of the creep vs. time diagram corresponding to secondary creep"@en .


###  http://fairmat-nfdi.eu/taxonomy/Misorientation
:Misorientation rdf:type owl:Class ;
                rdfs:subClassOf :TwoDDefect ;
                rdfs:comment "difference in crystallographic orientation between two crystallites in a polycrystalline material"@en .


###  http://fairmat-nfdi.eu/taxonomy/Morphology
:Morphology rdf:type owl:Class ;
            rdfs:subClassOf :StructuralProperty ;
            rdfs:comment "morphological data of materials of various shapes"@en .


###  http://fairmat-nfdi.eu/taxonomy/Name
:Name rdf:type owl:Class ;
      rdfs:subClassOf :StructuralProperty ;
      rdfs:comment "precursor name"@en .


###  http://fairmat-nfdi.eu/taxonomy/OneDDefect
:OneDDefect rdf:type owl:Class ;
            rdfs:subClassOf :StructuralProperty ;
            rdfs:comment "linear crystallographic defect or irregularity within a crystal structure which contains an abrupt change in the arrangement of atoms"@en .


###  http://fairmat-nfdi.eu/taxonomy/OpticalBandGap
:OpticalBandGap rdf:type owl:Class ;
                rdfs:subClassOf :OpticalProperty ;
                rdfs:comment "optical band gap obtained from the absorption spectrum"@en .


###  http://fairmat-nfdi.eu/taxonomy/OpticalProperty
:OpticalProperty rdf:type owl:Class ;
                 rdfs:subClassOf :MaterialProperty ;
                 rdfs:comment "opical properties of the materials"@en .


###  http://fairmat-nfdi.eu/taxonomy/OxidationPotential
:OxidationPotential rdf:type owl:Class ;
                    rdfs:subClassOf :ElectrochemPhaseStability ;
                    rdfs:comment "the oxidation potential (voltage vs. Li/Li+)"@en .


###  http://fairmat-nfdi.eu/taxonomy/Particle
:Particle rdf:type owl:Class ;
          rdfs:subClassOf :StructuralProperty ;
          rdfs:comment "Information of particulate materials_n"@en .


###  http://fairmat-nfdi.eu/taxonomy/PassivationCurrent
:PassivationCurrent rdf:type owl:Class ;
                    rdfs:subClassOf :CorrosionProperty ;
                    rdfs:comment "corrosion current at the passivation potential"@en .


###  http://fairmat-nfdi.eu/taxonomy/PassivationPotential
:PassivationPotential rdf:type owl:Class ;
                      rdfs:subClassOf :CorrosionProperty ;
                      rdfs:comment "corrosion potential, at which the corrosion current has a peak value, and above which there is a range of potentials, where the metal is in a passive state"@en .


###  http://fairmat-nfdi.eu/taxonomy/Permeability
:Permeability rdf:type owl:Class ;
              rdfs:subClassOf :MagneticProperty ;
              rdfs:comment "measure of magnetization that a material obtains in response to an applied magnetic field"@en .


###  http://fairmat-nfdi.eu/taxonomy/Permittivity
:Permittivity rdf:type owl:Class ;
              rdfs:subClassOf :ElectricalProperty ;
              rdfs:comment "measure of the electric polarizability of a material"@en .


###  http://fairmat-nfdi.eu/taxonomy/PhaseCrystalStructure
:PhaseCrystalStructure rdf:type owl:Class ;
                       rdfs:subClassOf :StructuralProperty ;
                       rdfs:comment "crystal structure of a phase_(n)"@en .


###  http://fairmat-nfdi.eu/taxonomy/Photoluminescence
:Photoluminescence rdf:type owl:Class ;
                   rdfs:subClassOf :OpticalProperty ;
                   rdfs:comment "light emission from any form of matter after the absorption of photons"@en .


###  http://fairmat-nfdi.eu/taxonomy/PiezoelectricChargeCoefficient
:PiezoelectricChargeCoefficient rdf:type owl:Class ;
                                rdfs:subClassOf :PiezoelectricProperty ;
                                rdfs:comment "electrical charge induced when polarized when stress is applied, presented by values assigned to symbols d_{ij}, i.e d_{11}, d_{22}, d_{33} etc."@en .


###  http://fairmat-nfdi.eu/taxonomy/PiezoelectricProperty
:PiezoelectricProperty rdf:type owl:Class ;
                       rdfs:subClassOf :MaterialProperty ;
                       rdfs:comment "property of certain materials which induces an electric field when mechanical stress is applied OR VICE VERSA"@en .


###  http://fairmat-nfdi.eu/taxonomy/PiezoelectricStrainCoefficient
:PiezoelectricStrainCoefficient rdf:type owl:Class ;
                                rdfs:subClassOf :PiezoelectricProperty ;
                                rdfs:comment "strain induced when polarized when electric field applied, presented by values assigned to symbols d*_{ij}, i.e d*_{11}, d*_{22}, d*_{33} etc."@en .


###  http://fairmat-nfdi.eu/taxonomy/PiezoelectricVoltageCoefficient
:PiezoelectricVoltageCoefficient rdf:type owl:Class ;
                                 rdfs:subClassOf :PiezoelectricProperty ;
                                 rdfs:comment "voltage induced when polarized when stress applied, presented by values assigned to symbols g_{ij}, i.e g_{11}, g_{22}, g_{33} etc."@en .


###  http://fairmat-nfdi.eu/taxonomy/PittingInitiationPotential
:PittingInitiationPotential rdf:type owl:Class ;
                            rdfs:subClassOf :CorrosionProperty ;
                            rdfs:comment "the lowest value of the corrosion potential at which pit initiation is possible on a passive surface in a given corrosive environment"@en .


###  http://fairmat-nfdi.eu/taxonomy/PlasticStrainRatio
:PlasticStrainRatio rdf:type owl:Class ;
                    rdfs:subClassOf :MechanicalProperty ;
                    rdfs:comment "ratio of true strain in the width direction over true strain in the thickness direction"@en .


###  http://fairmat-nfdi.eu/taxonomy/PoissonRatio
:PoissonRatio rdf:type owl:Class ;
              rdfs:subClassOf :MechanicalProperty ;
              rdfs:comment "ratio of transverse strain to corresponding axial strain on a material stressed along one axis"@en .


###  http://fairmat-nfdi.eu/taxonomy/PoralizedPotential
:PoralizedPotential rdf:type owl:Class ;
                    rdfs:subClassOf :CorrosionProperty ;
                    rdfs:comment "potential across the electrode/electrolyte interface that is the sum of the corrosion potential and the applied polarization"@en .


###  http://fairmat-nfdi.eu/taxonomy/PoreDiameter
:PoreDiameter rdf:type owl:Class ;
              rdfs:subClassOf :StructuralProperty ;
              rdfs:comment "pore diameters of materials"@en .


###  http://fairmat-nfdi.eu/taxonomy/PoreLimitingDiameter
:PoreLimitingDiameter rdf:type owl:Class ;
                      rdfs:subClassOf :StructuralProperty ;
                      rdfs:comment "diameter of the largest probe that can traverse through pore channels"@en .


###  http://fairmat-nfdi.eu/taxonomy/Porosity
:Porosity rdf:type owl:Class ;
          rdfs:subClassOf :StructuralProperty ;
          rdfs:comment "pore density of materials"@en .


###  http://fairmat-nfdi.eu/taxonomy/ReactivationPotential
:ReactivationPotential rdf:type owl:Class ;
                       rdfs:subClassOf :CorrosionProperty ;
                       rdfs:comment "corrosion potential below which reactivation takes place"@en .


###  http://fairmat-nfdi.eu/taxonomy/RealVolume
:RealVolume rdf:type owl:Class ;
            rdfs:subClassOf :StructuralProperty ;
            rdfs:comment "ratio of the two volumes = effetice volume / initial volume"@en .


###  http://fairmat-nfdi.eu/taxonomy/RedoxPotential
:RedoxPotential rdf:type owl:Class ;
                rdfs:subClassOf :CorrosionProperty ;
                rdfs:comment "potential of a reversible oxidation-reduction reaction in a given electrolyte recorded on a S.H.E. scale"@en .


###  http://fairmat-nfdi.eu/taxonomy/ReductionArea
:ReductionArea rdf:type owl:Class ;
               rdfs:subClassOf :MechanicalProperty ;
               rdfs:comment "proportional reduction of the cross-sectional area of a tensile test piece at the plane of fracture measured after fracture"@en .


###  http://fairmat-nfdi.eu/taxonomy/ReductionPotential
:ReductionPotential rdf:type owl:Class ;
                    rdfs:subClassOf :ElectrochemPhaseStability ;
                    rdfs:comment "the reduction potential (voltage vs. Li/Li+)"@en .


###  http://fairmat-nfdi.eu/taxonomy/Reflectance
:Reflectance rdf:type owl:Class ;
             rdfs:subClassOf :OpticalProperty ;
             rdfs:comment "ratio of the radiation flux reflected by a sample surface to the incident radiation flux"@en .


###  http://fairmat-nfdi.eu/taxonomy/RefractiveIndex
:RefractiveIndex rdf:type owl:Class ;
                 rdfs:subClassOf :OpticalProperty ;
                 rdfs:comment "ratio of the speed of the light in the vacuum to that in a material"@en .


###  http://fairmat-nfdi.eu/taxonomy/RemanentMagnetization
:RemanentMagnetization rdf:type owl:Class ;
                       rdfs:subClassOf :MagneticProperty ;
                       rdfs:comment "The magnetization that remains after magnetizing a ferromagnetic substance in a magnetic field and then removing the magnetic field"@en .


###  http://fairmat-nfdi.eu/taxonomy/RemanentPolarization
:RemanentPolarization rdf:type owl:Class ;
                      rdfs:subClassOf :FerroelectricProperty ;
                      rdfs:comment "polarization that remains after removing the electric field applied to an object, presented by values assigned to symbols P_{r}"@en .


###  http://fairmat-nfdi.eu/taxonomy/ResilienceModulus
:ResilienceModulus rdf:type owl:Class ;
                   rdfs:subClassOf :MechanicalProperty ;
                   rdfs:comment "measure of resilience modulus defined as the maximum energy that can be absorbed per unit volume without creating permanent distortion"@en .


###  http://fairmat-nfdi.eu/taxonomy/Resistivity
:Resistivity rdf:type owl:Class ;
             rdfs:subClassOf :ElectricalProperty ;
             rdfs:comment "quantity how strongly it resists electric current"@en .


###  http://fairmat-nfdi.eu/taxonomy/RheologicalProperty
:RheologicalProperty rdf:type owl:Class ;
                     rdfs:subClassOf :MaterialProperty ;
                     rdfs:comment "The material properties that govern the specific way in which materials deform or flowin response to applied forces or stresses"@en .


###  http://fairmat-nfdi.eu/taxonomy/RuptureTime
:RuptureTime rdf:type owl:Class ;
             rdfs:subClassOf :MechanicalProperty ;
             rdfs:comment "time necessary produce failure while materials is subjected to constant load at a constant temperature"@en .


###  http://fairmat-nfdi.eu/taxonomy/SaturationMagentization
:SaturationMagentization rdf:type owl:Class ;
                         rdfs:subClassOf :MagneticProperty ;
                         rdfs:comment "a state in which the magnetization inside a magnetic substance does noe increase any more even when the strength of the magnetic filed is increased or the magnetization strength of this state. Defined as the magnitude of magnetization moment per unit volume and per unit weight."@en .


###  http://fairmat-nfdi.eu/taxonomy/SaturationPolarization
:SaturationPolarization rdf:type owl:Class ;
                        rdfs:subClassOf :FerroelectricProperty ;
                        rdfs:comment "Maximum polarization when an electric field is applied to an object, presented by values assigned to symbols P_{s}"@en .


###  http://fairmat-nfdi.eu/taxonomy/Shape
:Shape rdf:type owl:Class ;
       rdfs:subClassOf :Particle ;
       rdfs:comment "Particle shape of material_n if it is particulate materials"@en .


###  http://fairmat-nfdi.eu/taxonomy/ShearModulus
:ShearModulus rdf:type owl:Class ;
              rdfs:subClassOf :MechanicalProperty ;
              rdfs:comment "measure of the elastic shear stiffness of a material and is defined as the ratio of shear stress to the shear strain"@en .


###  http://fairmat-nfdi.eu/taxonomy/Size
:Size rdf:type owl:Class ;
      rdfs:subClassOf :Particle ;
      rdfs:comment "Particle size of materials_n if it is particulate materials"@en .


###  http://fairmat-nfdi.eu/taxonomy/Soc
:Soc rdf:type owl:Class ;
     rdfs:subClassOf :ElectricalProperty ;
     rdfs:comment "spin-orbit coupling"@en .


###  http://fairmat-nfdi.eu/taxonomy/SpecificHeat
:SpecificHeat rdf:type owl:Class ;
              rdfs:subClassOf :ThermophysicalProperty ;
              rdfs:comment "heat capacity of a substance divided by mass"@en .


###  http://fairmat-nfdi.eu/taxonomy/SpinHallAngle
:SpinHallAngle rdf:type owl:Class ;
               rdfs:subClassOf :ElectricalProperty ;
               rdfs:comment "When a current is applied to a material with a very large spin-orbit interaction, the current does not go straight due to the strong spin-orbit interaction, and different spins diverge in the width direction on both sodes of the sample, resulting in spin accumumation and spin current. The ratio of the generated spin current to the flowed current."@en .


###  http://fairmat-nfdi.eu/taxonomy/SpinOrbitSplittingEnergy
:SpinOrbitSplittingEnergy rdf:type owl:Class ;
                          rdfs:subClassOf :ElectricalProperty ;
                          rdfs:comment "energy level splitting energy produced by the spin–orbit interaction of a particle's spin with its motion inside a potential"@en .


###  http://fairmat-nfdi.eu/taxonomy/Squareness
:Squareness rdf:type owl:Class ;
            rdfs:subClassOf :MagneticProperty ;
            rdfs:comment "A parameter indicating how close the shape of the hysteresis curve is to a square"@en .


###  http://fairmat-nfdi.eu/taxonomy/StackingFaultEnergy
:StackingFaultEnergy rdf:type owl:Class ;
                     rdfs:subClassOf :TwoDDefect ;
                     rdfs:comment "energy required to form irregularities in the sequence of crystlline planes"@en .


###  http://fairmat-nfdi.eu/taxonomy/StandardElectrodePotential
:StandardElectrodePotential rdf:type owl:Class ;
                            rdfs:subClassOf :CorrosionProperty ;
                            rdfs:comment "reversible potential for an electrode process when all products and reactants are at unit activity"@en .


###  http://fairmat-nfdi.eu/taxonomy/StandardState
:StandardState rdf:type owl:Class ;
               rdfs:subClassOf :ThermophysicalProperty ;
               rdfs:comment "reference state of a material(pure substance, mixture or solution) defined to calculate its properties under different conditions"@en .


###  http://fairmat-nfdi.eu/taxonomy/StandardStatePressure
:StandardStatePressure rdf:type owl:Class ;
                       rdfs:subClassOf :ThermophysicalProperty ;
                       rdfs:comment "pressure at which standard state of a material is defined"@en .


###  http://fairmat-nfdi.eu/taxonomy/StandardStateTemperature
:StandardStateTemperature rdf:type owl:Class ;
                          rdfs:subClassOf :ThermophysicalProperty ;
                          rdfs:comment "temperature at which standard state of a material is defined"@en .


###  http://fairmat-nfdi.eu/taxonomy/StorageModulus
:StorageModulus rdf:type owl:Class ;
                rdfs:subClassOf :VariableViscosity .


###  http://fairmat-nfdi.eu/taxonomy/StrainHardeningExponent
:StrainHardeningExponent rdf:type owl:Class ;
                         rdfs:subClassOf :MechanicalProperty ;
                         rdfs:comment "constant used in calculations relating to stress-strain bahavior in work hardening"@en .


###  http://fairmat-nfdi.eu/taxonomy/StressIntensityFactor
:StressIntensityFactor rdf:type owl:Class ;
                       rdfs:subClassOf :MechanicalProperty ;
                       rdfs:comment "magnitude of the mathematically ideal, crack-tip stress field for a particular mode in a homogeneous, linear-elastic body"@en .


###  http://fairmat-nfdi.eu/taxonomy/StressIntensityFactorRange
:StressIntensityFactorRange rdf:type owl:Class ;
                            rdfs:subClassOf :MechanicalProperty ;
                            rdfs:comment "variation in the stress intensity factor in a cycle in fatigue"@en .


###  http://fairmat-nfdi.eu/taxonomy/StructuralProperty
:StructuralProperty rdf:type owl:Class ;
                    rdfs:subClassOf :MaterialProperty ;
                    rdfs:comment "microscopic structure related properties"@en .


###  http://fairmat-nfdi.eu/taxonomy/SurfaceArea
:SurfaceArea rdf:type owl:Class ;
             rdfs:subClassOf :StructuralProperty ;
             rdfs:comment "Surface area of material_n"@en .


###  http://fairmat-nfdi.eu/taxonomy/Susceptibility
:Susceptibility rdf:type owl:Class ;
                rdfs:subClassOf :MagneticProperty ;
                rdfs:comment "a dimensionless proportionality constant that indicates the degree of magentic polarization of a material"@en .


###  http://fairmat-nfdi.eu/taxonomy/TemperatureCoefficientOfResistance
:TemperatureCoefficientOfResistance rdf:type owl:Class ;
                                    rdfs:subClassOf :ElectricalProperty ;
                                    rdfs:comment "a change in resistance per unit resistance per degree rise in temperature based upon the resistance of 0 degree celcius"@en .


###  http://fairmat-nfdi.eu/taxonomy/TensileProperty
:TensileProperty rdf:type owl:Class ;
                 rdfs:subClassOf :MechanicalProperty ;
                 rdfs:comment "properties indicate how the material will react to forces being applied in tension"@en .


###  http://fairmat-nfdi.eu/taxonomy/TensileStrength
:TensileStrength rdf:type owl:Class ;
                 rdfs:subClassOf :MechanicalProperty ;
                 rdfs:comment "maximum stress that can be applied to the material before it breaks"@en .


###  http://fairmat-nfdi.eu/taxonomy/ThermalConductivity
:ThermalConductivity rdf:type owl:Class ;
                     rdfs:subClassOf :ThermophysicalProperty ;
                     rdfs:comment "quantity of heat that passes in unit time through unit area of a substance"@en .


###  http://fairmat-nfdi.eu/taxonomy/ThermalDiffusivity
:ThermalDiffusivity rdf:type owl:Class ;
                    rdfs:subClassOf :ThermophysicalProperty ;
                    rdfs:comment "thermal conductivity divided by density and specific heat capacity at constant pressure"@en .


###  http://fairmat-nfdi.eu/taxonomy/ThermalExpansionCoefficient
:ThermalExpansionCoefficient rdf:type owl:Class ;
                             rdfs:subClassOf :ThermophysicalProperty ;
                             rdfs:comment "fractional change in size of a material in response to a change in temperature"@en .


###  http://fairmat-nfdi.eu/taxonomy/ThermophysicalProperty
:ThermophysicalProperty rdf:type owl:Class ;
                        rdfs:subClassOf :MaterialProperty ;
                        rdfs:comment "physical properties of materials affected by temperature, related to the structure and dynamics of atoms"@en .


###  http://fairmat-nfdi.eu/taxonomy/TimeTertiaryCreep
:TimeTertiaryCreep rdf:type owl:Class ;
                   rdfs:subClassOf :MechanicalProperty ;
                   rdfs:comment "time necessary to reach tertiary creep stage"@en .


###  http://fairmat-nfdi.eu/taxonomy/TotalElongation
:TotalElongation rdf:type owl:Class ;
                 rdfs:subClassOf :MechanicalProperty ;
                 rdfs:comment "percentage by which the material can be stretched before it breaks"@en .


###  http://fairmat-nfdi.eu/taxonomy/TotalPoreVolume
:TotalPoreVolume rdf:type owl:Class ;
                 rdfs:subClassOf :StructuralProperty ;
                 rdfs:comment "Total Pore volume of materials"@en .


###  http://fairmat-nfdi.eu/taxonomy/Toughness
:Toughness rdf:type owl:Class ;
           rdfs:subClassOf :MechanicalProperty ;
           rdfs:comment "The amount of energy a material can absorb before it fractures"@en .


###  http://fairmat-nfdi.eu/taxonomy/TransPassivationPotential
:TransPassivationPotential rdf:type owl:Class ;
                           rdfs:subClassOf :CorrosionProperty ;
                           rdfs:comment "corrosion potential above which the metal is in the transpassive state"@en .


###  http://fairmat-nfdi.eu/taxonomy/Transmittance
:Transmittance rdf:type owl:Class ;
               rdfs:subClassOf :OpticalProperty ;
               rdfs:comment "fraction of incident light which is transmitted"@en .


###  http://fairmat-nfdi.eu/taxonomy/TwoDDefect
:TwoDDefect rdf:type owl:Class ;
            rdfs:subClassOf :StructuralProperty ;
            rdfs:comment "planar defect separating two phases or crystal lattices, each of which may be solid, liquid, or gaseous"@en .


###  http://fairmat-nfdi.eu/taxonomy/UniformElongation
:UniformElongation rdf:type owl:Class ;
                   rdfs:subClassOf :MechanicalProperty ;
                   rdfs:comment "elongation at maximum load and immediately preceding the onset of necking in a tensile test"@en .


###  http://fairmat-nfdi.eu/taxonomy/UpperShelfEnergy
:UpperShelfEnergy rdf:type owl:Class ;
                  rdfs:subClassOf :MechanicalProperty ;
                  rdfs:comment "high fracture energy associated with ductile behavior"@en .


###  http://fairmat-nfdi.eu/taxonomy/VariableViscosity
:VariableViscosity rdf:type owl:Class ;
                   rdfs:subClassOf :RheologicalProperty ;
                   rdfs:comment "responce of fluid (slurry or liquid) resistance to a change in shape, or movement of neighbouring portions relative to one another by shear rate"@en .


###  http://fairmat-nfdi.eu/taxonomy/Velocity
:Velocity rdf:type owl:Class ;
          rdfs:subClassOf :OneDDefect ;
          rdfs:comment "Scan speed used for line scanning"@en .


###  http://fairmat-nfdi.eu/taxonomy/Viscosity
:Viscosity rdf:type owl:Class ;
           rdfs:subClassOf :RheologicalProperty ;
           rdfs:comment "How easily a liquid flows and is a measure of the fluid’s resistance to gradual deformation by shear forces."@en .


###  http://fairmat-nfdi.eu/taxonomy/Width
:Width rdf:type owl:Class ;
       rdfs:subClassOf :Particle ;
       rdfs:comment "width of the encapsulation layer"@en .


###  http://fairmat-nfdi.eu/taxonomy/YieldStengthCompressive
:YieldStengthCompressive rdf:type owl:Class ;
                         rdfs:subClassOf :MechanicalProperty ;
                         rdfs:comment "yield strength of material during compressive test"@en .


###  http://fairmat-nfdi.eu/taxonomy/YieldStrength
:YieldStrength rdf:type owl:Class ;
               rdfs:subClassOf :MechanicalProperty ;
               rdfs:comment "The stress value at which the plastic deformation of a material begins to occur"@en .


###  http://fairmat-nfdi.eu/taxonomy/YoungsModulus
:YoungsModulus rdf:type owl:Class ;
               rdfs:subClassOf :MechanicalProperty ;
               rdfs:comment "elastic properties of materials undergoing tension or compression in one direction"@en .


###  http://fairmat-nfdi.eu/taxonomy/ZeroDDefect
:ZeroDDefect rdf:type owl:Class ;
             rdfs:subClassOf :StructuralProperty ;
             rdfs:comment "defects that occur only at or around a single lattice point"@en .


###  http://fairmat-nfdi.eu/taxonomy/Phase_(n)
<http://fairmat-nfdi.eu/taxonomy/Phase_(n)> rdf:type owl:Class ;
                                            rdfs:subClassOf :StructuralProperty ;
                                            rdfs:comment "information of phase_n"@en .


###  Generated by the OWL API (version 4.5.25.2023-02-15T19:15:49Z) https://github.com/owlcs/owlapi
